theory/JITPer_load.thy
@@ -7,6 +7,162 @@ imports
 
 begin
 
+lemma length_of_addrmode_instr:
+  assumes a0:"xins = (Pmov_mr (Addrmode (Some R11) None 0) (bpf_to_x64_reg dst) chk)" and
+  a1:"l_bin = x64_encode xins" and
+  a2:"chk = M64"
+  shows "length l_bin = 4"
+proof-
+  let "?a" = "(Addrmode (Some R11) None 0)"
+  let "?r1" =  "(bpf_to_x64_reg dst)"
+  let "?c" = "chk"
+  have b1:"construct_rex_to_u8 (?c = M64) (and (u8_of_ireg ?r1) 0b1000 \<noteq> 0) False (and (u8_of_ireg R11) 0b1000 \<noteq> 0) \<noteq> 0x40"
+    using a2 apply(unfold construct_rex_to_u8_def Let_def bitfield_insert_u8_def u8_of_bool_def,simp_all) 
+    apply(cases "and (u8_of_ireg (bpf_to_x64_reg dst)) (8::8 word) \<noteq> (0::8 word)",simp_all)
+    done
+  have b3:"l_bin = (case ?a of Addrmode (Some rb) None dis \<Rightarrow> 
+      let (rex::u8) = ( construct_rex_to_u8 \<comment> \<open> WRXB \<close>
+        (?c = M64) \<comment> \<open> W \<close>
+        (and (u8_of_ireg ?r1) 0b1000 \<noteq> 0) \<comment> \<open> R \<close>
+        False \<comment> \<open> X \<close>
+        (and (u8_of_ireg rb) 0b1000 \<noteq> 0) \<comment> \<open> B \<close>
+        ) in
+        let (dis::u8) = scast dis in
+        let (rop::u8) = construct_modsib_to_u8 0b01 (u8_of_ireg ?r1) (u8_of_ireg rb) in
+        ([rex, 0x89, rop, dis]))" using b1 using a0 a1 x64_encode_def a2 by(cases chk,simp_all)
+  thus ?thesis by simp
+qed
+
+
+lemma load_m64_one_step_match_reg_1:
+  assumes a0:"(SBPF_OK pc' rs' m') = sbpf_step prog (SBPF_OK pc rs m)" and
+    a1:"xst = (Next xpc xrs xm)" and
+    a2:"match_state (SBPF_OK pc rs m) (pc,xst)" and
+    a3:"prog \<noteq> [] \<and> unat pc < length prog \<and> unat pc \<ge> 0" and
+    a4:"prog!(unat pc) = BPF_LDX chk dst src off" and
+    a5:"chk = M64"
+  shows "\<exists> somev. loadv M64 xm (Vlong (scast off + xrs (IR (bpf_to_x64_reg src)))) = Some (Vlong somev)"
+proof-
+  have c0:"\<forall> mc addr v. (Mem.loadv mc m (Vlong addr) = Some v) \<longrightarrow> (Mem.loadv mc xm (Vlong addr) = Some v)"
+    using a1 a2 match_state_def match_mem_def by simp
+  have c1:"xrs (IR (bpf_to_x64_reg src)) = rs (src)" using match_state_def match_reg_def a2 a1 by simp
+  have "\<exists> x. Mem.loadv chk m (Vlong ((rs src) + (scast off)))= Some x" 
+    using a0 a3 a4 a5 eval_load_def
+    using option.exhaust by fastforce 
+  then obtain x where b0:"Mem.loadv chk m (Vlong ((rs src) + (scast off)))= Some x"by auto
+  let "?off" = " ((rs src) + (scast off))"
+  have b1:"Mem.loadv chk m (Vlong ?off) = (option_val_of_u64 chk (option_u64_of_u8_8 (m 0 ?off) (m 0 (?off+1)) (m 0 (?off+2)) (m 0 (?off+3))
+                        (m 0 (?off+4)) (m 0 (?off+5)) (m 0 (?off+6)) (m 0 (?off+7)) ))"using a5 loadv_def by simp
+  let "?tmpres" = "(option_val_of_u64 chk (option_u64_of_u8_8 (m 0 ?off) (m 0 (?off+1)) (m 0 (?off+2)) (m 0 (?off+3))
+                        (m 0 (?off+4)) (m 0 (?off+5)) (m 0 (?off+6)) (m 0 (?off+7))))"
+  have b2_1:"?tmpres \<noteq> None" using b1 b0 option_val_of_u64_def memory_chunk_value_of_u64_def
+    by (metis option.distinct(1))
+  have b2:"\<exists> v. ?tmpres = Some (Vlong v)" using b2_1 memory_chunk_value_of_u64_def a5 
+    by (metis (no_types, lifting) memory_chunk.simps(16) option.case_eq_if option_val_of_u64_def)
+  then obtain v where b3:"?tmpres = Some (Vlong v)" by auto
+  have b4:"Vlong v = x" using b3 b0 b1 by simp
+  have b5:"Mem.loadv chk xm (Vlong ?off) = Some (Vlong v)" using b4 c0 b0 by blast
+  have c2:"Mem.loadv chk xm (Vlong (xrs (IR (bpf_to_x64_reg src)) + (scast off))) = Some (Vlong v)" using b0 c1 b5 by presburger
+  thus ?thesis using a5 add.commute by metis
+qed
+
+
+lemma load_m64_one_step_match_reg_2:
+  "(SBPF_OK pc' rs' m') = sbpf_step prog (SBPF_OK pc rs m) \<Longrightarrow>
+    xst = (Next xpc xrs xm) \<Longrightarrow>
+    match_state (SBPF_OK pc rs m) (pc,xst) \<Longrightarrow>
+    prog \<noteq> [] \<and> unat pc < length prog \<and> unat pc \<ge> 0 \<Longrightarrow>
+    prog!(unat pc) = BPF_LDX chk dst src off  \<Longrightarrow>
+    loadv M64 xm (Vlong (scast off + xrs (IR (bpf_to_x64_reg src)))) = Some (Vbyte x2) \<Longrightarrow>
+    chk = M64 \<Longrightarrow> False"
+  using load_m64_one_step_match_reg_1 by fastforce
+
+lemma val_type_unique2:"x = Vlong v \<longrightarrow> x \<notin> {Vshort (ucast v), Vint (ucast v)}"
+  by blast
+
+lemma load_m64_one_step_match_reg_3:
+  "(SBPF_OK pc' rs' m') = sbpf_step prog (SBPF_OK pc rs m) \<Longrightarrow>
+    xst = (Next xpc xrs xm) \<Longrightarrow>
+    match_state (SBPF_OK pc rs m) (pc,xst) \<Longrightarrow>
+    prog \<noteq> [] \<and> unat pc < length prog \<and> unat pc \<ge> 0 \<Longrightarrow>
+    prog!(unat pc) = BPF_LDX chk dst src off  \<Longrightarrow>
+    loadv M64 xm (Vlong (scast off + xrs (IR (bpf_to_x64_reg src)))) = Some (Vshort x2) \<Longrightarrow>
+    chk = M64 \<Longrightarrow> False"
+  using load_m64_one_step_match_reg_1 by fastforce
+
+lemma load_m64_one_step_match_reg_4:
+  "(SBPF_OK pc' rs' m') = sbpf_step prog (SBPF_OK pc rs m) \<Longrightarrow>
+    xst = (Next xpc xrs xm) \<Longrightarrow>
+    match_state (SBPF_OK pc rs m) (pc,xst) \<Longrightarrow>
+    prog \<noteq> [] \<and> unat pc < length prog \<and> unat pc \<ge> 0 \<Longrightarrow>
+    prog!(unat pc) = BPF_LDX chk dst src off  \<Longrightarrow>
+    loadv M64 xm (Vlong (scast off + xrs (IR (bpf_to_x64_reg src)))) = Some (Vint x2) \<Longrightarrow>
+    chk = M64 \<Longrightarrow> False"
+  using load_m64_one_step_match_reg_1  by fastforce
+
+lemma load_m64_one_step_match_reg_5:
+  "(SBPF_OK pc' rs' m') = sbpf_step prog (SBPF_OK pc rs m) \<Longrightarrow>
+    xst = (Next xpc xrs xm) \<Longrightarrow>
+    match_state (SBPF_OK pc rs m) (pc,xst) \<Longrightarrow>
+    prog \<noteq> [] \<and> unat pc < length prog \<and> unat pc \<ge> 0 \<Longrightarrow>
+    prog!(unat pc) = BPF_LDX chk dst src off  \<Longrightarrow>
+    loadv M64 xm (Vlong (scast off + xrs (IR (bpf_to_x64_reg src)))) = Some (Vptr x1 x2) \<Longrightarrow>
+    chk = M64 \<Longrightarrow> False"
+  using load_m64_one_step_match_reg_1  by fastforce
+
+lemma load_M64_one_step_match_reg:
+  " (SBPF_OK pc' rs' m') = sbpf_step prog (SBPF_OK pc rs m) \<Longrightarrow>
+    xst = (Next xpc xrs xm) \<Longrightarrow>
+    match_state (SBPF_OK pc rs m) (pc,xst) \<Longrightarrow>
+    prog \<noteq> [] \<and> unat pc < length prog \<and> unat pc \<ge> 0 \<Longrightarrow>
+    chk = M64 \<Longrightarrow>
+    prog!(unat pc) = BPF_LDX chk dst src off  \<Longrightarrow>
+    loadv M64 xm (Vlong (scast off + xrs (IR (bpf_to_x64_reg src)))) = Some (Vlong x5) \<Longrightarrow>
+    chk = M64 \<Longrightarrow>
+    match_reg rs' 
+    ((\<lambda>a::preg. 
+        if a = IR REG_SCRATCH then scast off + xrs (IR (bpf_to_x64_reg src)) 
+        else if a = IR REG_SCRATCH then scast off
+        else xrs a)
+    (IR (bpf_to_x64_reg dst) := x5)) "
+  apply (simp add: match_state_def match_reg_def eval_load_def)
+  using bpf_to_x64_reg_corr reg_r11_consist reg_rsp_consist
+  by (smt (z3) add.commute fun_upd_apply match_mem_def option.case_eq_if option.collapse option.sel sbpf_state.distinct(3) sbpf_state.inject(1) val.simps(40)) 
+
+
+lemma load_M64_one_step_match_mem:
+  "(SBPF_OK pc' rs' m') = sbpf_step prog (SBPF_OK pc rs m) \<Longrightarrow>
+    xst = (Next xpc xrs xm) \<Longrightarrow>
+    match_state (SBPF_OK pc rs m) (pc,xst) \<Longrightarrow>
+    prog \<noteq> [] \<and> unat pc < length prog \<and> unat pc \<ge> 0 \<Longrightarrow>
+    loadv M64 xm (Vlong (scast off + xrs (IR (bpf_to_x64_reg src)))) = Some (Vlong x5) \<Longrightarrow>
+    chk = M64 \<Longrightarrow>
+    prog!(unat pc) = BPF_LDX chk dst src off  \<Longrightarrow>
+    match_mem m' xm"
+  apply (simp add: match_state_def eval_load_def) 
+  by (metis (no_types, lifting) option.case_eq_if sbpf_state.inject(1) sbpf_state.simps(6))
+  
+
+
+lemma load_M64_one_step_match_stack:
+  "(SBPF_OK pc' rs' m') = sbpf_step prog (SBPF_OK pc rs m) \<Longrightarrow>
+    xst = (Next xpc xrs xm) \<Longrightarrow>
+    match_state (SBPF_OK pc rs m) (pc,xst) \<Longrightarrow>
+    prog \<noteq> [] \<and> unat pc < length prog \<and> unat pc \<ge> 0 \<Longrightarrow>
+    loadv M64 xm (Vlong (scast off + xrs (IR (bpf_to_x64_reg src)))) = Some (Vlong x5) \<Longrightarrow>
+    chk = M64 \<Longrightarrow>
+    prog!(unat pc) = BPF_LDX chk dst src off  \<Longrightarrow>
+    match_stack ((\<lambda>a::preg. 
+      if a = IR REG_SCRATCH then scast off + xrs (IR (bpf_to_x64_reg src)) 
+      else if a = IR REG_SCRATCH then scast off 
+      else xrs a)
+     (IR (bpf_to_x64_reg dst) := x5)) xm"
+  apply (simp add: match_state_def match_stack_def eval_alu_def eval_reg_def)
+  using reg_rsp_consist by blast
+
+
+
+
 lemma load_one_step1:
  assumes a0:"s' = sbpf_step prog s" and
   a1:"s = (SBPF_OK pc rs m)" and
@@ -15,9 +171,145 @@ lemma load_one_step1:
   a4:"match_state s (pc,xst)" and
   a5:"jitper prog = Some x64_prog" and                      
   a6:"prog \<noteq> [] \<and> unat pc < length prog \<and> unat pc \<ge> 0" and
-  a8:"prog!(unat pc) = BPF_LDX chk dst sop off" 
+  a8:"prog!(unat pc) = BPF_LDX chk dst src off" and
+  a9:"chk = M64"
 shows "\<exists> xst'. x64_sem1 1 x64_prog (pc,xst) = (pc',xst') \<and> 
   match_state s' (pc',xst')"
-    
+  
+(* 1. as BPF_ADD generates a single list of jited x64 assembly, so we only need one step  *)
+  apply(subgoal_tac "\<exists>xst'::outcome. one_step x64_prog (pc, xst) = (pc', xst') \<and> match_state s' (pc', xst')")
+  subgoal
+    by auto
+  subgoal
+    apply (unfold one_step_def Let_def)
+(* 2. according to the code structure of JITPer, removing the first case statement *)
+    apply(subgoal_tac "x64_prog ! unat (fst (pc, xst)) = the (per_jit_load_reg64 dst src chk off)")
+     prefer 2
+    subgoal
+      using a5 a6 a8 aux5 per_jit_ins_def by fastforce
+    subgoal
+      apply (subgoal_tac "the (per_jit_load_reg64 dst src chk off) = (3, 0, x64_encode(Pmovq_ri R11 (scast off))@x64_encode (Paddq_rr R11 (bpf_to_x64_reg src))@
+    x64_encode (Pmov_mr (Addrmode (Some R11) None 0) (bpf_to_x64_reg dst) chk))")
+       prefer 2
+      subgoal by (simp add: per_jit_load_reg64_def Let_def)
+      apply (subgoal_tac "(x64_encode(Pmovq_ri R11 (scast off))@x64_encode (Paddq_rr R11 (bpf_to_x64_reg src))@
+    x64_encode (Pmov_mr (Addrmode (Some R11) None 0) (bpf_to_x64_reg dst) chk)) !1 \<noteq> 0x39")
+       prefer 2
+      subgoal apply(unfold x64_encode_def) 
+        apply(cases "Pmovq_ri REG_SCRATCH (scast off)",simp_all)
+        using x64_encode_def construct_rex_to_u8_def bitfield_insert_u8_def Let_def
+        by simp
+      subgoal
+        unfolding a3
+        apply simp
+        apply (erule subst)
+        apply (erule subst)
+(* 3. here we get a simplified version, next step is to run the 6 x64 assembly one by one *)
+(* 3.1 *)
+        apply (subgoal_tac "Suc 2 = (3::nat)") prefer 2 subgoal by simp
+        apply (erule subst [of _ 3])
+        apply (simp only: x64_sem.simps)
+        apply simp
+(* 3.1.1 using consistency to get x64 assembly *)
+        apply (subgoal_tac "x64_decode (0::nat)
+            (x64_encode(Pmovq_ri R11 (scast off))@x64_encode (Paddq_rr R11 (bpf_to_x64_reg src))@
+    x64_encode (Pmov_mr (Addrmode (Some R11) None 0) (bpf_to_x64_reg dst) chk))
+            = Some (10, Pmovq_ri REG_SCRATCH (scast off))")
+         prefer 2
+        subgoal
+          apply (rule_tac l_bin = "x64_encode (Pmovq_ri REG_SCRATCH (scast off))" in x64_encode_decode_consistency)
+          subgoal using list_in_list_prop
+            using list_in_list_concat by blast
+          subgoal by simp
+          subgoal using x64_encode_def construct_rex_to_u8_def bitfield_insert_u8_def Let_def u8_list_of_u64_def
+            by auto
+          done
+        apply simp
+        apply (erule subst)
+        apply (simp add: exec_instr_def)
+(* 3.2 *)
+        apply (subgoal_tac "Suc 1 = (2::nat)") prefer 2 subgoal by simp
+        apply (erule subst [of _ 2])
+        apply (simp only: x64_sem.simps)
+        apply simp
+        apply (subgoal_tac "x64_decode (10::nat)
+            (x64_encode(Pmovq_ri R11 (scast off))@x64_encode (Paddq_rr R11 (bpf_to_x64_reg src))@
+    x64_encode (Pmov_mr (Addrmode (Some R11) None 0) (bpf_to_x64_reg dst) chk))
+            = Some (3, Paddq_rr R11 (bpf_to_x64_reg src))")
+         prefer 2
+(* this is necessary for later list_in_list_prop_aux2 *)
+        apply (subgoal_tac "length (x64_encode (Pmovq_ri REG_SCRATCH (scast off))) = 10")
+         prefer 2 subgoal using x64_encode_def construct_rex_to_u8_def bitfield_insert_u8_def Let_def u8_list_of_u64_def by auto
+        subgoal
+          apply (rule_tac l_bin = "x64_encode (Paddq_rr R11 (bpf_to_x64_reg src))" in x64_encode_decode_consistency)
+          subgoal using list_in_list_prop_aux2
+            by metis 
+          subgoal by simp
+          subgoal apply (erule subst) 
+            using x64_encode_def construct_rex_to_u8_def bitfield_insert_u8_def Let_def
+            by fastforce
+          done
+        apply simp
+        apply (erule subst)
+        apply (simp add: exec_instr_def)
 
+(* 3.3 *)
+        apply (subgoal_tac "Suc 0 = (1::nat)") prefer 2 subgoal by simp
+        apply (erule_tac subst [of _ 1])
+        apply (simp only: x64_sem.simps)
+        (*apply simp*)
+(* using consistency to get x64 assembly *)
+        apply (subgoal_tac "x64_decode (13::nat)
+            (x64_encode(Pmovq_ri R11 (scast off))@x64_encode (Paddq_rr R11 (bpf_to_x64_reg src))@
+    x64_encode (Pmov_mr (Addrmode (Some R11) None 0) (bpf_to_x64_reg dst) chk))
+            = Some (4, Pmov_mr (Addrmode (Some R11) None 0) (bpf_to_x64_reg dst) chk)")
+         prefer 2
+(* this is necessary for later list_in_list_prop_aux2 *)
+        apply (subgoal_tac "length ((x64_encode(Pmovq_ri R11 (scast off))@x64_encode (Paddq_rr R11 (bpf_to_x64_reg src)))) = 13")
+         prefer 2 subgoal using x64_encode_def construct_rex_to_u8_def bitfield_insert_u8_def Let_def u8_list_of_u64_def by auto
+        subgoal
+          apply (rule_tac l_bin = "x64_encode (Pmov_mr (Addrmode (Some R11) None 0) (bpf_to_x64_reg dst) chk)" in x64_encode_decode_consistency)
+          subgoal using list_in_list_prop_aux2
+            by (metis (no_types, opaque_lifting) append_eq_append_conv2)
+          subgoal by simp
+          subgoal using length_of_addrmode_instr a9 by simp done
+        apply simp
+        apply (erule subst)
+        apply (simp add: exec_instr_def exec_load_def eval_addrmode64_def Let_def)
+        apply(subgoal_tac "bpf_to_x64_reg src \<noteq> REG_SCRATCH") 
+         prefer 2 subgoal using reg_r11_consist by blast
+         apply (rule conjI)
+         apply (rule impI)
+         apply simp
+        apply(rule impI)
+        using a9 apply(cases chk,simp_all)
+        
+(* 4. now we get exec_instr (one step of x64 add assembly), we prove the \<and>, first left, then right *)
+         apply (rule conjI)
+        subgoal
+          using a0 a1 a2 a5 a6 a8 corr_pc_aux2 insert_iff prod_cases3 by metis
+        unfolding a1 a2
+(* 4.1  match_reg *)
+         apply (simp add: match_state_def)
+         apply(cases "loadv M64 xm (Vlong (scast off + xrs (IR (bpf_to_x64_reg src))))",simp_all)
+        subgoal using load_m64_one_step_match_reg_1 a0 a1 a2 a3 a4 a5 a6 a8 a9 by (metis option.discI) 
+        subgoal for a using a9 apply (cases a,simp_all) 
+          subgoal using load_m64_one_step_match_reg_1 a0 a1 a2 a3 a4 a5 a6 a8 a9 apply (metis option.sel val.distinct(7)) done
+          subgoal for x2 using load_m64_one_step_match_reg_2 a0 a1 a2 a3 a4 a5 a6 a8 a9 by metis
+          subgoal for x3 using load_m64_one_step_match_reg_3 a0 a1 a2 a3 a4 a5 a6 a8 a9 by metis
+          subgoal for x4 using load_m64_one_step_match_reg_4 a0 a1 a2 a3 a4 a5 a6 a8 a9 by metis
+           prefer 2 subgoal for x61 x62 using load_m64_one_step_match_reg_5 a0 a1 a2 a3 a4 a5 a6 a8 a9 by metis
+          subgoal for x5 
+            apply(rule conjI)
+            using load_M64_one_step_match_reg a0 a1 a2 a3 a4 a5 a6 a8 a9 apply auto[1]
+(* 4.2  match_mem *)
+            apply(rule conjI)
+            using load_M64_one_step_match_mem a0 a1 a2 a3 a4 a5 a6 a8 a9 apply metis
+(* 4.3  match_stack *)
+            using load_M64_one_step_match_stack a0 a1 a2 a3 a4 a5 a6 a8 a9 by auto
+          done
+        done
+      done
+    done
+  done
 end
